src/program_proof/lockservice/proof.v
@@ -18,41 +18,6 @@ Context `{!heapG Σ}.
 Implicit Types s : Slice.t.
 Implicit Types (stk:stuckness) (E: coPset).
 
-Record TryLockArgsC :=
-  mkTryLockArgsC{
-  Lockname:u64;
-  CID:u64;
-  Seq:u64
-  }.
-Instance: Settable TryLockArgsC := settable! mkTryLockArgsC <Lockname; CID; Seq>.
-
-Record TryLockReplyC :=
-  mkTryLockReplyC {
-  OK:bool ;
-  Stale:bool
-  }.
-Instance: Settable TryLockReplyC := settable! mkTryLockReplyC <OK; Stale>.
-Instance TryLockArgs_rpc : RPCRequest TryLockArgsC := {getCID x := x.(CID); getSeq x := x.(Seq)}.
-
-
-Definition own_lockreply (args_ptr:loc) (lockReply:TryLockReplyC): iProp Σ :=
-  "HreplyOK" ∷ args_ptr ↦[TryLockReply.S :: "OK"] #lockReply.(OK)
-  ∗ "HreplyStale" ∷ args_ptr ↦[TryLockReply.S :: "Stale"] #lockReply.(Stale)
-.
-
-#[refine] Instance trylock_rpc : RPCReply TryLockReplyC TryLockReply.S := { own_reply := own_lockreply }.
-Proof.
-  iIntros (rloc) "Halloc".
-  iDestruct (struct_fields_split with "Halloc") as "(HOK&HStale&_) /=".
-  iExists {| OK:=_ ; Stale:=_ |}; iFrame.
-Defined.
-
-Global Instance ToVal_bool : into_val.IntoVal bool.
-Proof.
-  refine {| into_val.to_val := λ (x: bool), #x;
-            IntoVal_def := false; |}; congruence.
-Defined.
-
 Definition locknameN (lockname : u64) := nroot .@ "lock" .@ lockname.
 
   Context `{!mapG Σ (u64*u64) (option bool)}.
@@ -78,238 +43,46 @@ Definition TryLock_Post : TryLockArgsC -> bool -> iProp Σ := λ args reply, (�
 Definition TryLock_Pre : TryLockArgsC -> iProp Σ := λ _, True%I.
 Definition TryLockRequest_inv := RPCRequest_inv TryLock_Pre TryLock_Post.
 
-Definition LockServer_mutex_inv (srv:loc) (γrpc:RPC_GS) : iProp Σ :=
-  ∃ (lastSeq_ptr lastReply_ptr locks_ptr:loc) (lastSeqM:gmap u64 u64)
-    (lastReplyM locksM:gmap u64 bool),
-      "HlastSeqOwn" ∷ srv ↦[LockServer.S :: "lastSeq"] #lastSeq_ptr
-    ∗ "HlastReplyOwn" ∷ srv ↦[LockServer.S :: "lastReply"] #lastReply_ptr
-    ∗ "HlocksOwn" ∷ srv ↦[LockServer.S :: "locks"] #locks_ptr
-
-    ∗ "HlastSeqMap" ∷ is_map (lastSeq_ptr) lastSeqM
-    ∗ "HlastReplyMap" ∷ is_map (lastReply_ptr) lastReplyM
-    ∗ "HlocksMap" ∷ is_map (locks_ptr) locksM
-    ∗ ("Hlockeds" ∷ [∗ map] ln ↦ locked ; _ ∈ locksM ; validLocknames, (⌜locked=true⌝ ∨ (Ps ln)))
-    
-    ∗ ("Hsrpc" ∷ RPCServer_own lastSeqM lastReplyM γrpc)
-.
-
-(* Should make this readonly so it can be read by the RPC background thread *)
-Definition read_lock_args (args_ptr:loc) (lockArgs:TryLockArgsC): iProp Σ :=
-  "#HLocknameValid" ∷ ⌜is_Some (validLocknames !! lockArgs.(Lockname))⌝
-  ∗ "#HSeqPositive" ∷ ⌜int.nat lockArgs.(Seq) > 0⌝
-  ∗ "#HTryLockArgsOwnLockname" ∷ readonly (args_ptr ↦[TryLockArgs.S :: "Lockname"] #lockArgs.(Lockname))
-  ∗ "#HTryLockArgsOwnCID" ∷ readonly (args_ptr ↦[TryLockArgs.S :: "CID"] #lockArgs.(CID))
-  ∗ "#HTryLockArgsOwnSeq" ∷ readonly (args_ptr ↦[TryLockArgs.S :: "Seq"] #lockArgs.(Seq))
-.
-
-Definition replycacheinvN : namespace := nroot .@ "replyCacheInvN".
-Definition mutexN : namespace := nroot .@ "lockservermutexN".
-Definition lockRequestInvN (cid seq : u64) := nroot .@ "lock" .@ cid .@ "," .@ seq.
-
-Definition is_lockserver (srv_ptr:loc) γrpc: iProp Σ :=
-  ∃ mu_ptr,
-      "Hmuptr" ∷ readonly (srv_ptr ↦[LockServer.S :: "mu"] #mu_ptr)
-    ∗ ( "Hlinv" ∷ inv replycacheinvN (ReplyCache_inv γrpc ) )
-    ∗ ( "Hmu" ∷ is_lock mutexN #mu_ptr (LockServer_mutex_inv srv_ptr γrpc))
-.
-
 Definition TryLock_spec_pre (srv args reply:loc) (lockArgs:TryLockArgsC) γrpc γPost : iProp Σ
   :=
-    "#Hls" ∷ is_lockserver srv γrpc 
+     "#Hls" ∷ is_lockserver srv γrpc (Ps:=Ps)
            ∗ "#HargsInv" ∷ inv rpcRequestInvN (TryLockRequest_inv lockArgs γrpc γPost)
-           ∗ "#Hargs" ∷ read_lock_args args lockArgs.
+           ∗ "#Hargs" ∷ read_args args lockArgs.
 
-Lemma TryLock_spec (srv args reply:loc) (lockArgs:TryLockArgsC) (lockReply:TryLockReplyC) γrpc γPost :
+Lemma tryLock_core_spec (srv args:loc) (lockArgs:TryLockArgsC) :
+{{{ 
+     LockServer_own_core srv (Ps:=Ps) ∗ TryLock_Pre lockArgs
+}}}
+  LockServer__tryLock_core #srv #args
+{{{
+   v, RET v; LockServer_own_core srv (Ps:=Ps)
+      ∗ (∃b:bool, ⌜v = #b⌝ ∗ TryLock_Post lockArgs b)
+}}}.
+Proof.
+Admitted.
+
+Lemma TryLock_spec_using_generic (srv args reply:loc) (lockArgs:TryLockArgsC) (lockReply:TryLockReplyC) γrpc γPost :
 {{{ TryLock_spec_pre srv args reply lockArgs γrpc γPost
-    ∗ "Hreply" ∷ own_reply reply lockReply
+    ∗ own_reply reply lockReply
 }}}
   LockServer__TryLock #srv #args #reply
 {{{ RET #false; ∃ lockReply', own_reply reply lockReply'
     ∗ ((⌜lockReply'.(Stale) = true⌝ ∗ RPCRequestStale lockArgs γrpc)
   ∨ RPCReplyReceipt lockArgs lockReply'.(OK) γrpc)
 }}}.
-Proof using Type*.
-  iIntros (Φ) "[Hpre Hreply] HPost".
-  iNamed "Hpre".
-  iNamed "Hargs"; iNamed "Hreply".
-  unfold own_lockreply. iNamed "Hreply".
-  wp_lam.
-  wp_pures.
-  iNamed "Hls".
-  wp_loadField.
-  wp_apply (acquire_spec mutexN #mu_ptr _ with "Hmu").
-  iIntros "(Hlocked & Hlsown)".
-  iNamed "Hlsown".
-  wp_seq.
-  repeat wp_loadField.
-  wp_apply (wp_MapGet with "HlastSeqMap").
-  iIntros (v ok) "(HSeqMapGet&HlastSeqMap)"; iDestruct "HSeqMapGet" as %HSeqMapGet.
-  wp_pures.
-  wp_storeField.
-
-  iAssert
-    (
-{{{
-readonly (args ↦[TryLockArgs.S :: "Seq"] #lockArgs.(Seq))
-∗ ⌜int.nat lockArgs.(Seq) > 0⌝
-}}}
-  if: #ok then #v ≥ struct.loadF TryLockArgs.S "Seq" #args
-         else #false
-{{{ ifr, RET ifr; ∃b:bool, ⌜ifr = #b⌝
-  ∗ ((⌜b = false⌝ ∗ ⌜int.nat v < int.nat lockArgs.(Seq)⌝)
-      ∨
-     (⌜b = true⌝ ∗  ⌜(int.val lockArgs.(Seq) ≤ int.val v ∧ ok=true)%Z⌝)
-    )
-}}}
-    )%I as "Htemp".
-  {
-    iIntros (Ψ). iModIntro.
-    iIntros "HΨpre HΨpost".
-    iDestruct "HΨpre" as "[#Hseq %]".
-    destruct ok.
-    { wp_pures. wp_loadField. wp_binop.
-      destruct bool_decide eqn:Hineq.
-      - apply bool_decide_eq_true in Hineq.
-        iApply "HΨpost". iExists true.
-        iSplitL ""; first done.
-        iRight. iFrame. by iPureIntro.
-      - apply bool_decide_eq_false in Hineq.
-        iApply "HΨpost". iExists false.
-        iSplitL ""; first done.
-        iLeft. iFrame. iSplitL ""; eauto.
-        iPureIntro. lia.
-    }
-    {
-      iMod (fmcounter_map_alloc 0 _ lockArgs.(CID) with "[$]") as "Hlseq_own_new".
-      wp_pures.
-      apply map_get_false in HSeqMapGet as [Hnone Hv]. rewrite Hv.
-      iApply "HΨpost". iExists false.
-      iSplitL ""; first done.
-      iLeft. iSplitL ""; eauto.
-    }
-  }
-  wp_apply ("Htemp" with "[]"); eauto.
-  iIntros (ifr) "Hifr".
-  iDestruct "Hifr" as (b ->) "Hifr".
-  destruct b.
-  - (* cache hit *)
-    iDestruct "Hifr" as "[[% _]|[_ Hineq ]]"; first discriminate.
-    iDestruct "Hineq" as %[Hineq Hok].
-    rewrite ->Hok in *.
-    apply map_get_true in HSeqMapGet.
-    wp_pures. repeat wp_loadField. wp_binop.
-    destruct bool_decide eqn:Hineqstrict.
-      { (* Stale case *)
-        wp_pures. wp_storeField. wp_loadField.
-        apply bool_decide_eq_true in Hineqstrict.
-        iMod (smaller_seqno_stale_fact with "[] Hsrpc") as "[Hsrpc #Hstale]"; eauto.
-        wp_apply (release_spec mutexN #mu_ptr _ with "[-HPost HreplyOK HreplyStale]"); iFrame; iFrame "#".
-        { (* Re-establish LockServer_mutex_inv *)
-          iNext. iExists _, _, _, _,_,_. iFrame "#". iFrame.
-        }
-        wp_seq. iApply "HPost". iExists ({| OK := lockReply.(OK); Stale := true |}); iFrame.
-        iLeft.
-        iFrame "Hstale". by iFrame.
-      }
-      (* Not stale *)
-      assert (v = lockArgs.(Seq)) as ->. {
-        (* not strict + non-strict ineq ==> eq *)
-        apply bool_decide_eq_false in Hineqstrict.
-        assert (int.val lockArgs.(Seq) = int.val v) by lia; word.
-      }
-      wp_pures.
-      repeat wp_loadField.
-      wp_apply (wp_MapGet with "HlastReplyMap").
-      iIntros (reply_v reply_get_ok) "(HlastReplyMapGet & HlastReplyMap)"; iDestruct "HlastReplyMapGet" as %HlastReplyMapGet.
-      wp_storeField.
-      iMod (server_replies_to_request with "[Hlinv] [HargsInv] [Hsrpc]") as "[#Hreceipt Hsrpc]"; eauto.
-      wp_loadField.
-      wp_apply (release_spec mutexN #mu_ptr _ with "[-HPost HreplyOK HreplyStale]"); iFrame; iFrame "#".
-      {
-        iNext. iExists _,_,_,_,_,_; iFrame "#"; iFrame.
-      }
-      wp_seq. iApply "HPost". iExists {| OK:=_; Stale:=_ |}; iFrame.
-      iRight. simpl. iFrame "#".
-    - (* cache miss *)
-      iDestruct "Hifr" as "[[_ Hineq ]|[% _]]"; last discriminate.
-      iDestruct "Hineq" as %Hineq.
-      rename Hineq into HnegatedIneq.
-      assert (int.val lockArgs.(Seq) > int.val v)%Z as Hineq; first lia.
-      wp_pures.
-      wp_loadField.
-      wp_loadField.
-      wp_loadField.
-      wp_apply (wp_MapInsert _ _ lastSeqM _ lockArgs.(Seq) (#lockArgs.(Seq)) with "HlastSeqMap"); try eauto.
-      iIntros "HlastSeqMap".
-      wp_pures.
-      wp_loadField.
-      wp_loadField.
-      wp_apply (wp_MapGet with "HlocksMap").
-      iIntros (lock_v ok2) "(HLocksMapGet&HlocksMap)"; iDestruct "HLocksMapGet" as %HLocksMapGet.
-      wp_pures.
-      destruct lock_v.
-      + (* Lock already held by someone *)
-        wp_pures.
-        wp_storeField.
-        repeat wp_loadField.
-        wp_apply (wp_MapInsert _ _ lastReplyM _ false #false with "HlastReplyMap"); first eauto; iIntros "HlastReplyMap".
-        wp_seq. wp_loadField.
-        iMod (server_processes_request _ _ _ _ _ false with "[Hlinv] [HargsInv] [] [Hsrpc]") as "(#Hrcptsoro & Hsrpc)"; eauto.
-        { simpl. injection HSeqMapGet. intros. rewrite H0. eauto. }
-        { by iLeft. }
-        wp_apply (release_spec mutexN #mu_ptr _ with "[-HreplyOK HreplyStale HPost]"); try iFrame "Hmu Hlocked".
-        {
-          iNext. iExists _, _, _, _, _, _; iFrame; iFrame "#".
-        }
-        wp_seq. iApply "HPost". iExists {| OK:=_; Stale:= _|}; iFrame.
-        iRight. iFrame "#".
-      + (* Lock not previously held by anyone *)
-        wp_pures.
-        wp_storeField.
-        repeat wp_loadField.
-        wp_apply (wp_MapInsert with "HlocksMap"); first eauto; iIntros "HlocksMap".
-        wp_seq. repeat wp_loadField.
-        wp_apply (wp_MapInsert with "HlastReplyMap"); first eauto; iIntros "HlastReplyMap".
-        wp_seq. wp_loadField.
-
-        iDestruct "HLocknameValid" as %HLocknameValid.
-        iDestruct (big_sepM2_dom with "Hlockeds") as %HlocksDom.
-        iDestruct (big_sepM2_delete _ _ _ lockArgs.(Lockname) false () with "Hlockeds") as "[HP Hlockeds]".
-        {
-          rewrite /map_get in HLocksMapGet.
-          assert (is_Some (locksM !! lockArgs.(Lockname))) as HLocknameInLocks.
-          { apply elem_of_dom. apply elem_of_dom in HLocknameValid. rewrite HlocksDom. done. }
-          destruct HLocknameInLocks as [ x  HLocknameInLocks].
-          rewrite HLocknameInLocks in HLocksMapGet.
-            by injection HLocksMapGet as ->.
-            (* TODO: Probably a better proof for this *)
-        }
-        { destruct HLocknameValid as [x HLocknameValid]. by destruct x. }
-        iDestruct (big_sepM2_insert_delete _ _ _ lockArgs.(Lockname) true () with "[$Hlockeds]") as "Hlockeds"; eauto.
-        iDestruct "HP" as "[%|HP]"; first discriminate.
-
-        iMod (server_processes_request _ _ _ _ _ true with "Hlinv HargsInv [HP] Hsrpc") as "(#Hrcptsoro & Hlseq_own & #Hrcagree2)"; eauto.
-        { simpl. apply pair_equal_spec in HSeqMapGet as [Hv _]. rewrite Hv. lia. }
-        { by iRight. }
-        replace (<[lockArgs.(Lockname):=()]> validLocknames) with (validLocknames).
-        2:{
-          rewrite insert_id; eauto. destruct HLocknameValid as [x HLocknameValid]. by destruct x.
-        }
-
-        wp_apply (release_spec mutexN #mu_ptr _ with "[-HreplyOK HreplyStale HPost]"); try iFrame "Hmu Hlocked".
-        {
-          iNext. iExists _, _, _, _, _, _; iFrame; iFrame "#".
-        }
-        wp_seq. iApply "HPost". iExists {| OK:=_; Stale:= _|}; iFrame.
-        iRight. iFrame "#".
-        Grab Existential Variables.
-        1: done.
-Admitted.
+Proof.
+  replace (LockServer__TryLock) with (LockServer_Function LockServer__tryLock_core "LockServer_TryLock" TryLockReply.S TryLockArgs.S); eauto.
+  iIntros (Φ) "Hpre Hpost".
+  iApply (LockServer_Function_spec with "[Hpre]"); eauto.
+  { refine tryLock_core_spec. }
+  iDestruct "Hpre" as  "[Hpre Hreply]".
+  iFrame.
+Qed.
 
 Lemma CallTryLock_spec (srv args reply:loc) (lockArgs:TryLockArgsC) (lockReply:TryLockReplyC) γrpc γPost :
-{{{ "#Hls" ∷ is_lockserver srv γrpc
+{{{ "#Hls" ∷ is_lockserver srv γrpc (Ps:=Ps)
     ∗ "#HargsInv" ∷ inv rpcRequestInvN (TryLockRequest_inv lockArgs γrpc γPost)
-    ∗ "#Hargs" ∷ read_lock_args args lockArgs
+    ∗ "#Hargs" ∷ read_args args lockArgs
     ∗ "Hreply" ∷ own_reply reply lockReply
 }}}
   CallTryLock #srv #args #reply
@@ -323,7 +96,7 @@ Lemma CallTryLock_spec (srv args reply:loc) (lockArgs:TryLockArgsC) (lockReply:T
 Proof using Type*.
   replace (CallTryLock) with (CallFunction LockServer__TryLock "CallTryLock" TryLockReply.S); eauto.
   iIntros (Φ) "Hpre Hpost".
-  iApply (CallFunction_spec with "[Hpre]"); eauto; try refine TryLock_spec; eauto.
+  iApply (CallFunction_spec with "[Hpre]"); eauto; try refine TryLock_spec_using_generic; eauto.
   { by rewrite /Persistent; eauto. }
   { Opaque own_reply. simpl. iNamed "Hpre". iFrame "#";iFrame. }
 Qed.
@@ -332,7 +105,7 @@ Lemma Clerk__TryLock_spec ck (srv:loc) (ln:u64) γrpc :
   {{{
        ⌜is_Some (validLocknames !! ln)⌝
       ∗ own_clerk ck srv γrpc
-      ∗ is_lockserver srv γrpc
+      ∗ is_lockserver srv γrpc (Ps:=Ps)
   }}}
     Clerk__TryLock ck #ln
   {{{ v, RET v; ∃(b:bool), ⌜v = #b⌝ ∗ own_clerk ck srv γrpc ∗ (⌜b = false⌝ ∨ Ps ln) }}}.
@@ -366,21 +139,23 @@ Proof using Type*.
   iIntros (reply) "Hreply".
   wp_pures.
   iDestruct "Hsrv" as (mu_ptr) "Hsrv". iNamed "Hsrv".
-  iMod (alloc_γrc {| CID:=cid; Seq:=cseqno; Lockname:=ln |} _ TryLock_Pre TryLock_Post with "[Hlinv] [Hcseq_own] []") as "[Hcseq_own HallocPost]"; eauto.
+  iMod (alloc_γrc (mkTryLockArgsC ln cid cseqno) _ TryLock_Pre TryLock_Post with "[Hlinv] [Hcrpc] []") as "[Hcseq_own HallocPost]"; eauto.
+  { simpl. admit. }
   iDestruct "HallocPost" as (γP) "[#Hreqinv_init HγP]".
+  Print TryLockArgsC.
   wp_apply (wp_forBreak
               (fun b =>
- (let lockArgs := {| CID:=cid; Seq:=cseqno; Lockname:=ln |} in
-    "#Hargs" ∷ read_lock_args args lockArgs
+ (let lockArgs := (mkTryLockArgsC ln cid cseqno) in
+    "#Hargs" ∷ read_args args lockArgs
   ∗ "#Hargsinv" ∷ (inv rpcRequestInvN (TryLockRequest_inv lockArgs γrpc γP))
   ∗ "Hcid" ∷ ck_l ↦[Clerk.S :: "cid"] #cid
-  ∗ "Hseq" ∷ (ck_l ↦[Clerk.S :: "seq"] #(LitInt (word.add lockArgs.(Seq) 1)))
+  ∗ "Hseq" ∷ (ck_l ↦[Clerk.S :: "seq"] #(LitInt (word.add lockArgs.(getSeq) 1)))
   ∗ "Hprimary" ∷ ck_l ↦[Clerk.S :: "primary"] #srv
   ∗ "Hargs_ptr" ∷ args_ptrs ↦[refT (uint64T * (uint64T * (uint64T * unitT))%ht)] #args
   ∗ "Herrb_ptr" ∷ (∃ (err:bool), errb_ptr ↦[boolT] #err)
-  ∗ "Hreply" ∷ (∃ lockReply, own_lockreply reply lockReply ∗ (⌜b = true⌝ ∨ (⌜lockReply.(OK) = false⌝ ∨ Ps ln)))
+  ∗ "Hreply" ∷ (∃ lockReply, own_reply reply lockReply ∗ (⌜b = true⌝ ∨ (⌜lockReply.(OK) = false⌝ ∨ Ps ln)))
   ∗ "HγP" ∷ (⌜b = false⌝ ∨ own γP (Excl ()))
-  ∗ ("Hcseq_own" ∷ cid fm[[γrpc.(cseq)]]↦(int.nat lockArgs.(Seq) + 1))
+  ∗ ("Hcseq_own" ∷ cid fm[[γrpc.(cseq)]]↦(int.nat lockArgs.(getSeq) + 1))
   ∗ ("HΦpost" ∷ ∀ v : val, (∃ rb : bool, ⌜v = #rb⌝ ∗ own_clerk #ck_l srv γrpc ∗ (⌜rb = false⌝ ∨ Ps ln)) -∗ Φ v)
               ))%I with "[] [-]"); eauto.
   {
@@ -421,7 +196,7 @@ Proof using Type*.
       wp_load.
       iDestruct "HγP" as "[%|HγP]"; first discriminate.
       iDestruct "HCallPost" as "[ [_ Hbad] | #Hrcptstoro]"; simpl.
-      { iDestruct (fmcounter_map_agree_strict_lb with "Hcseq_own Hbad") as %bad. lia. }
+      { iDestruct (fmcounter_map_agree_strict_lb with "Hcseq_own Hbad") as %bad. simpl in bad. lia. }
       iMod (get_request_post with "Hargsinv Hrcptstoro HγP") as "HP".
       wp_pures.
       iNamed "Hreply".
@@ -434,7 +209,7 @@ Proof using Type*.
   }
   {
     iFrame; iFrame "#".
-    iSplitL ""; first done.
+    iSplitL ""; eauto.
     iSplitL "Herrb_ptr"; eauto.
     iDestruct (struct_fields_split with "Hreply") as "(?& ? & _)".
     iExists {| OK:=false; Stale:=false |}. iFrame. by iLeft.
